\documentclass[../ana2u.tex]{subfiles}
\begin{document}
\setcounter{section}{1}

\section{Beispiele für Integrale}
\begin{bsp}
    \( \integral{x}{0}{1} \).\\
    %Bild Treppenfunktion 1/n, 2/n...
    \( g_n = \frac{1}{n} \lfloor nx \rfloor \) 
    konvergiert gleichmäßig in \( [0,1] \)
    gegen \(x\) auf \( [\frac{ k-1 }{n}, \frac{k}{n}) \)
    ist \( g_n(x) = \frac{k-1}{n} \).
    \[ x_k = \frac{k}{n},
    \quad x_k - x_{k-1} = \frac{1}{n} \]

    \begin{align*}
        \Rightarrow \integral{g_n(x)}{0}{1}
        &= \sum_{k=1}^n \frac{k-1}{n} \cdot \frac{1}{n}\\
        &= \frac{1}{n^2} \cdot \frac{n(n-1)}{2} \\
        &= \frac{1}{2} (1-\frac{1}{n}) 
        \overset{n\rightarrow \infty}{\rightarrow} 
        \frac{1}{2}
    \end{align*}
    \[ \Rightarrow \integral{x}{0}{1} = \frac{1}{2} \]
\end{bsp}
\begin{bsp}
    \begin{beh}
        \( f(x) = \exp x \) auf \( [a,b] \).
    \end{beh}    
    Wollen zeigen:
    \[ \integral{\exp x}{a}{b} = \exp b - \exp a. \]
    \begin{bew}
        Setze \( x_k = a + \frac{k}{n} (b-a) \)
        \[ g_n(x) = \begin{cases}
            \exp(x_{k-1}), &x_{k-1} \leq x < x_k\\
            \exp b, &x = b
        \end{cases}. \]
        
        \begin{align*}
            \Rightarrow \integral{g_n(x)}{a}{b} 
            &= \sum_{k=1}^n \exp x_{k-1}(x_k-x_k-1)\\
            &= \sum_{k=1}^n 
            \exp\left(a + \frac{(k-1)(b-a)}{n}\right)
            \frac{b-a}{n}\\
            &= \frac{b-a}{n} \exp a \cdot 
            \sum_{k=1}^n \underbrace{\exp \left( (k-1) \frac{b-a}{n} \right)}_
            {= \exp \left( \frac{b-a}{n} \right)^{k-1} := \;q^{k-1}}\\
            &= \frac{b-a}{n} \exp a \cdot 
            \underbrace{\sum_{k=1}^n q^{k-1} }_{\text{geom. Summe}}\\
            &= \frac{ b-a }{n} \exp a 
            \frac{ \exp(\frac{b-a}{n})^n - 1}{ \exp(\frac{b-a}{n}) - 1 }\\
            &= \frac{\frac{b-a}{n}}{\exp \left( \frac{b-a}{n} \right) - 1}
            \cdot \underbrace{\exp a (\exp(b-a) - 1)}_{=\exp b - \exp a}\\
            &\overset{n \rightarrow \infty}{\longrightarrow} 
            1 \cdot (\exp b - \exp a) = \exp b - \exp a.
        \end{align*}
    \end{bew}
\end{bsp}
\end{document}